proof_checking/pxl_core_meta_validation_v3/pxl_meta_sets_v3/coq/PXL_Deep_Soundness.v
@@ -31,7 +31,7 @@ Record frame := {
 
 Definition valuation (F:frame) := nat -> (W F) -> Prop.
 
-Fixpoint eval (F:frame) (v:valuation F) (w:(W F)) (φ:form) : Prop :=
+Fixpoint eval (F:frame) (v:valuation F) (w:W F) (φ:form) {struct φ} : Prop :=
   match φ with
   | Bot      => False
   | Var n    => v n w
@@ -44,7 +44,7 @@ Fixpoint eval (F:frame) (v:valuation F) (w:(W F)) (φ:form) : Prop :=
   end.
 
 Definition valid_on (F:frame) (φ:form) : Prop :=
-  forall v w, eval F v w φ.
+  forall (v:valuation F) (w:W F), eval F v w φ.
 
 (* Proof system *)
 Inductive Prov : form -> Prop :=
@@ -60,26 +60,26 @@ Inductive Prov : form -> Prop :=
 | nec   : forall p, Prov p -> Prov (Box p).
 
 (* Soundness of axioms and rules *)
-Lemma sound_K : forall F v w p q,
+Lemma sound_K : forall (F:frame) (v:valuation F) (w:W F) (p q:form),
   eval F v w (Impl (Box (Impl p q)) (Impl (Box p) (Box q))).
 Proof.
-  intros F v w p q Hb Hp u Hwu. apply Hb in Hwu. apply Hwu. apply Hp in Hwu. exact Hwu.
+  intros F v w p q Hb Hp u Hwu.
+  exact ((Hb u Hwu) (Hp u Hwu)).
 Qed.
 
-Lemma sound_T : forall F v w p,
+Lemma sound_T : forall (F:frame) (v:valuation F) (w:W F) (p:form),
   eval F v w (Impl (Box p) p).
 Proof.
   intros F v w p Hb. apply Hb. apply (R_refl F).
-Qed;
+Qed.
 
-
-Lemma sound_4 : forall F v w p,
+Lemma sound_4 : forall (F:frame) (v:valuation F) (w:W F) (p:form),
   eval F v w (Impl (Box p) (Box (Box p))).
 Proof.
   intros F v w p Hb u Hwu t Hut. apply Hb. eapply (R_trans F); eauto.
 Qed.
 
-Lemma sound_5 : forall F v w p,
+Lemma sound_5 : forall (F:frame) (v:valuation F) (w:W F) (p:form),
   eval F v w (Impl (Dia p) (Box (Dia p))).
 Proof.
   intros F v w p [u [Hwu Hpu]] t Hwt. exists u. split.
@@ -87,48 +87,47 @@ Proof.
   - exact Hpu.
 Qed.
 
-Lemma sound_PL_imp : forall F v w p q r,
+Lemma sound_PL_imp : forall (F:frame) (v:valuation F) (w:W F) (p q r:form),
   eval F v w (Impl (Impl p q) (Impl (Impl q r) (Impl p r))).
 Proof.
   intros F v w p q r Hpqr Hqr Hp. apply Hqr. apply Hpqr. exact Hp.
 Qed.
 
-Lemma sound_PL_and1 : forall F v w p q,
+Lemma sound_PL_and1 : forall (F:frame) (v:valuation F) (w:W F) (p q:form),
   eval F v w (Impl (And p q) p).
 Proof.
   intros F v w p q [Hp _]. exact Hp.
 Qed.
 
-Lemma sound_PL_and2 : forall F v w p q,
+Lemma sound_PL_and2 : forall (F:frame) (v:valuation F) (w:W F) (p q:form),
   eval F v w (Impl (And p q) q).
 Proof.
   intros F v w p q [_ Hq]. exact Hq.
 Qed.
 
-Lemma sound_mp : forall F v w p q,
+Lemma sound_mp : forall (F:frame) (p q:form),
   valid_on F (Impl p q) -> valid_on F p -> valid_on F q.
 Proof.
-  intros F v w p q Hpq Hp. apply (Hpq v w). apply (Hp v w).
+  intros F p q Hpq Hp v w. exact ((Hpq v w) (Hp v w)).
 Qed.
 
-Lemma sound_nec : forall F p,
+Lemma sound_nec : forall (F:frame) (p:form),
   valid_on F p -> valid_on F (Box p).
 Proof.
   intros F p H v w u Hwu. apply (H v u).
 Qed.
 
-Theorem soundness : forall (F:frame) φ, Prov φ -> valid_on F φ.
-Proof.
-  intros F φ H. induction H.
-  - intros v w. apply sound_K.
-  - intros v w. apply sound_T.
-  - intros v w. apply sound_4.
-  - intros v w. apply sound_5.
-  - intros v w. apply sound_PL_imp.
-  - intros v w. apply sound_PL_and1.
-  - intros v w. apply sound_PL_and2.
-  - apply sound_mp; assumption.
-  - apply sound_nec; assumption.
-Qed.
+Fixpoint soundness (F:frame) (φ:form) (H:Prov φ) : valid_on F φ :=
+  match H in Prov φ return valid_on F φ with
+  | ax_K p q => fun v w => sound_K F v w p q
+  | ax_T p => fun v w => sound_T F v w p
+  | ax_4 p => fun v w => sound_4 F v w p
+  | ax_5 p => fun v w => sound_5 F v w p
+  | ax_PL_imp p q r => fun v w => sound_PL_imp F v w p q r
+  | ax_PL_and1 p q => fun v w => sound_PL_and1 F v w p q
+  | ax_PL_and2 p q => fun v w => sound_PL_and2 F v w p q
+  | mp p q H1 H2 => fun v w => sound_mp F p q (soundness F (Impl p q) H1) (soundness F p H2) v w
+  | nec p H1 => fun v w => sound_nec F p (soundness F p H1) v w
+  end.
 
 End Deep.
